data_to_word_assign: fix data_to_word_assign proof (add the assumption that ffi names cannot be "MappedRead" or "MappedWrite" for assign_thm)

compiler/backend/proofs/data_to_word_assignProofScript.sml
@@ -12821,8 +12821,15 @@ Proof
   \\ fs [make_cons_ptr_def,get_lowerbits_def]
 QED
 
+Definition not_mapped_ffi_name_def:
+  not_mapped_ffi_name n <=>
+    (n <> "MappedRead" /\ n <> "MappedWrite")
+End
+
 Theorem assign_FFI:
-   (?n. op = FFI n) ==> ^assign_thm_goal
+   (?n. op = FFI n /\
+      not_mapped_ffi_name n) ==>
+   ^assign_thm_goal
 Proof
   rpt strip_tac \\ drule0 (evaluate_GiveUp |> GEN_ALL) \\ rw [] \\ fs []
   \\ `t.termdep <> 0` by fs[]
@@ -12890,6 +12897,7 @@ Proof
   \\ simp[]
   \\ qpat_abbrev_tac`ex1 = if ffi_name = "" then _ else _`
   \\ qpat_abbrev_tac`ex2 = if ffi_name = "" then _ else _`
+  \\ fs[not_mapped_ffi_name_def]
   \\ IF_CASES_TAC >- ( fs[shift_def] )
   \\ simp[wordSemTheory.get_var_def,lookup_insert]
   \\ qpat_x_assum`¬_`kall_tac
@@ -13238,6 +13246,7 @@ QED
 
 Theorem assign_FFI_final:
    state_rel c l1 l2 s (t:('a,'c,'ffi) wordSem$state) [] locs /\
+   not_mapped_ffi_name i /\
    (op_requires_names (FFI i) ==> names_opt <> NONE) /\
    cut_state_opt names_opt s = SOME x /\
    get_vars args x.locals = SOME vals /\
@@ -13304,6 +13313,7 @@ Proof
   \\ IF_CASES_TAC >- ( fs[shift_def] )
   \\ simp[wordSemTheory.get_var_def,lookup_insert]
   \\ qpat_x_assum`¬_`kall_tac
+  \\ fs[not_mapped_ffi_name_def]
   \\ BasicProvers.TOP_CASE_TAC
   >- (
     `F` suffices_by rw[]
@@ -13714,8 +13724,13 @@ Proof[exclude_simps = EXP_LE_LOG_SIMP EXP_LT_LOG_SIMP LE_EXP_LOG_SIMP
   \\ qexists_tac ‘x.space − LENGTH y2’ \\ fs []
 QED
 
+Definition not_mapped_ffi_def:
+  not_mapped_ffi (op: op) <=>
+    (op <> FFI "MappedRead" /\ op <> FFI "MappedWrite")
+End
+
 Theorem assign_thm:
-   ^assign_thm_goal
+  not_mapped_ffi op ==> ^assign_thm_goal
 Proof
   Cases_on `op = AllocGlobal` \\ fs []
   THEN1 (fs [do_app] \\ every_case_tac \\ fs [])
@@ -13723,11 +13738,12 @@ Proof
   THEN1 (fs [do_app] \\ every_case_tac \\ fs [])
   \\ Cases_on `op = GreaterEq` \\ fs []
   THEN1 (fs [do_app] \\ every_case_tac \\ fs [])
+  \\ simp[not_mapped_ffi_def] \\ strip_tac
   \\ map_every (fn th =>
          (Cases_on `^(th |> concl |> dest_imp |> #1)` THEN1 (fs []
              \\ match_mp_tac th \\ fs [])))
       (DB.match ["-"] ``_ ==> ^assign_thm_goal`` |> map (#1 o #2))
-  \\ fs [] \\ strip_tac
+  \\ fs [not_mapped_ffi_name_def] \\ strip_tac
   \\ Cases_on`op = CopyByte T` >- (
     fs[do_app_def,do_space_def,do_app_aux_def]
     \\ every_case_tac \\ fs[] )
